complete with the Acc(essibility) approach which is a bit shorter in this case

theories/ackermann/ackermann.v
@@ -60,7 +60,7 @@ Fixpoint ack_pwc m n (d : Dack m n) : sig (Gack m n).
 Proof.
   refine(match m, n return Dack m n → sig (Gack m n) with
   |   0 , _   => λ _, exist _ (1+n) _
-  | S m ,   0 => λ d, let (o,ho) := ack_pwc m 1 (Dack_pi1 d) in 
+  | S m ,   0 => λ d, let (o,ho) := ack_pwc m 1 (Dack_pi1 d)     in
                       exist _ o _
   | S m , S n => λ d, let (v,hv) := ack_pwc (S m) n (Dack_pi2 d) in
                       let (o,ho) := ack_pwc m v (Dack_pi3 d hv)  in
@@ -117,5 +117,54 @@ Proof. eauto. Qed.
 (* Extraction is right on spot *)
 Extraction Inline ack_pwc.
 Extraction ack.
+
+(* This alternate avoids tailored small inversions and
+   replaces them with the generic Acc_inv, so we get
+   a shorter proof.*)
+
+(* We define the sub-call/call relation inductivelly *)
+Inductive ack_sub_calls : nat*nat → nat*nat → Prop :=
+  | ack_sc_1 m     : ack_sub_calls (m,1) (S m,0)
+  | ack_sc_2 m n   : ack_sub_calls (S m,n) (S m, S n)
+  | ack_sc_3 m n v : Gack (S m) n v → ack_sub_calls (m,v) (S m,S n).
+
+#[local] Hint Constructors ack_sub_calls : core.
+
+Arguments Acc_inv {_ _ _} _ {_}.
+
+(* We use Acc_inv that recover the sub-term for a proof of d : Acc ... *) 
+Fixpoint ack_pwc_Acc m n (d : Acc ack_sub_calls (m,n)) : sig (Gack m n).
+Proof.
+  refine(match m, n return Acc ack_sub_calls (m,n) → sig (Gack m n) with
+  |   0 , _   => λ _, exist _ (1+n) _
+  | S m ,   0 => λ d, let (o,ho) := ack_pwc_Acc m 1 (Acc_inv d _)     in
+                      exist _ o _
+  | S m , S n => λ d, let (v,hv) := ack_pwc_Acc (S m) n (Acc_inv d _) in
+                      let (o,ho) := ack_pwc_Acc m v (Acc_inv d _)     in
+                      exist _ o _
+  end d); eauto.
+Defined.
+
+Lemma ack_sub_calls_inv p q : 
+       ack_sub_calls p q 
+     → match q with
+       | (  0 ,   n) => False
+       | (S m ,   0) => (m,1) = p
+       | (S m , S n) => (S m, n) = p
+                      ∨ ∃v, Gack (S m) n v
+                          ∧ (m,v) = p
+       end.
+Proof. destruct 1; eauto. Qed. 
+
+Lemma ack_termination_Acc m n : Acc ack_sub_calls (m,n).
+Proof.
+  induction m in n |- *; [ | induction n ];
+    constructor. 
+  1,2: intros ? []%ack_sub_calls_inv; auto.
+  intros ? [ | (? & _ & ?)]%ack_sub_calls_inv; subst; auto.
+Qed.
+
+(* Then we can finish as in the case of Dack *)
+
 
 
